Tweaks in SpaceAdjMat 1/2/3

graph/SpaceAdjMatGraph2.v
@@ -174,13 +174,13 @@ Section SpaceAdjMatGraph2.
       + rewrite (Zlength_concat _ size); trivial; lia.
   Qed.
 
-  Definition SpaceAdjMatGraph' sh (f : E -> E) g_contents gaddr : mpred :=
+  Definition SpaceAdjMatGraph' sh g_contents gaddr : mpred :=
     data_at sh (tarray tint (size * size))
             (map Vint (map Int.repr g_contents))
             gaddr.
 
   Definition SpaceAdjMatGraph sh (f : E -> E) g gaddr : mpred :=
-    SpaceAdjMatGraph' sh f (graph_to_list g f) gaddr.
+    SpaceAdjMatGraph' sh (graph_to_list g f) gaddr.
 
 (*
   The below is not currently used by SpaceDijkGraph because 
